move JournalAppend from CommitterAppendImpl.i.dfy into CommitterImpl.i.dfy

Impl/CommitterAppendImpl.i.dfy
@@ -16,29 +16,28 @@ module CommitterAppendImpl {
   import opened StateModel
   import opened IOModel
   import CommitterAppendModel
-  import opened CommitterImpl
   import JournalistImpl
 
-  method JournalAppend(
-      cm: Committer,
-      key: Key, value: Value)
-  requires cm.Inv()
-  requires cm.status == CommitterModel.StatusReady
-  requires JournalistModel.canAppend(
-    cm.journalist.I(), JournalInsert(key, value))
-  modifies cm.Repr
-  ensures cm.Inv()
-  ensures forall o | o in cm.Repr :: o in old(cm.Repr) || fresh(o)
-  ensures cm.I() == CommitterAppendModel.JournalAppend(
-      old(cm.I()), key, value)
-  {
-    CommitterAppendModel.reveal_JournalAppend();
-    cm.reveal_ReprInv();
+//   method JournalAppend(
+//       cm: Committer,
+//       key: Key, value: Value)
+//   requires cm.Inv()
+//   requires cm.status == CommitterModel.StatusReady
+//   requires JournalistModel.canAppend(
+//     cm.journalist.I(), JournalInsert(key, value))
+//   modifies cm.Repr
+//   ensures cm.Inv()
+//   ensures forall o | o in cm.Repr :: o in old(cm.Repr) || fresh(o)
+//   ensures cm.I() == CommitterAppendModel.JournalAppend(
+//       old(cm.I()), key, value)
+//   {
+//     CommitterAppendModel.reveal_JournalAppend();
+//     cm.reveal_ReprInv();
 
-    var je := JournalInsert(key, value);
-    cm.journalist.append(je);
+//     var je := JournalInsert(key, value);
+//     cm.journalist.append(je);
 
-    cm.Repr := {cm} + cm.syncReqs.Repr + cm.journalist.Repr;
-    cm.reveal_ReprInv();
-  }
+//     cm.Repr := {cm} + cm.syncReqs.Repr + cm.journalist.Repr;
+//     cm.reveal_ReprInv();
+//   }
 }
